get stuff to run

disk-betree/ImplFlushPolicy.i.dfy
@@ -76,11 +76,13 @@ module ImplFlushPolicy {
 
   method getActionToFlush(k: ImplConstants, s: ImplVariables, stack: seq<BT.G.Reference>, slots: seq<uint64>) returns (action : ImplModelFlushPolicy.Action)
   requires |stack| <= 40
-  requires ImplModelFlushPolicy.ValidStackSlots(Ic(k), IVars(s), stack, slots)
   requires Inv(k, s)
+  requires ImplModelFlushPolicy.ValidStackSlots(Ic(k), IVars(s), stack, slots)
   decreases 0x1_0000_0000_0000_0000 - |stack|
   ensures action == ImplModelFlushPolicy.getActionToFlush(Ic(k), IVars(s), stack, slots)
   {
+    ImplModelFlushPolicy.reveal_getActionToFlush();
+
     if |stack| as uint64 == 40 {
       action := ImplModelFlushPolicy.ActionFail;
     } else {
@@ -104,17 +106,12 @@ module ImplFlushPolicy {
             KMTable.kmtableSeqWeightEq(child.buckets);
             var childTotalWeight: uint64 := KMTable.computeWeightKMTableSeq(child.buckets);
 
-            var extraRootWeight: uint64;
-            if ref == BT.G.Root() {
-              extraRootWeight := WeightBucket(s.rootBucket);
-            } else {
-              extraRootWeight := 0;
-            }
+            var extraRootWeight: uint64 := if ref == BT.G.Root() then s.rootBucketWeightBound else 0;
 
             if slotWeight + childTotalWeight + extraRootWeight <= MaxTotalBucketWeight() as uint64 {
               action := ImplModelFlushPolicy.ActionFlush(ref, slot);
             } else {
-              action := ImplModelFlushPolicy.getActionToFlush(k, s, stack + [childref], slots + [slot]);
+              action := getActionToFlush(k, s, stack + [childref], slots + [slot]);
             }
           } else {
             action := ImplModelFlushPolicy.getActionToPageIn(s.cache, childref);
@@ -126,227 +123,47 @@ module ImplFlushPolicy {
     }
   }
 
-  /*
-  lemma getActionToSplitValidAction(k: Constants, s: Variables, stack: seq<BT.G.Reference>, slots: seq<uint64>, i: uint64)
-  requires 0 <= i as int < |stack|
+  method runFlushPolicy(k: ImplConstants, s: ImplVariables, io: DiskIOHandler)
+  returns (s' : Variables)
   requires Inv(k, s)
-  requires ValidStackSlots(k, s, stack, slots)
-  requires forall j | 0 <= j < |stack| :: stack[j] in s.ephemeralIndirectionTable
-  requires forall j | 0 <= j < |stack| - 1 :: s.cache[stack[j]].children.value[slots[j]] == stack[j+1]
-  requires forall j | 1 <= j < |stack| :: stack[j] != BT.G.Root()
-  requires s.cache[stack[|stack| - 1]].children.Some? ==> |s.cache[stack[|stack| - 1]].buckets| >= 2
-  requires i as int < |stack| - 1 ==> |s.cache[stack[i]].buckets| >= MaxNumChildren()
-  ensures ValidAction(k, s, getActionToSplit(k, s, stack, slots, i))
-  ensures var action := getActionToSplit(k, s, stack, slots, i);
-      action.ActionGrow? || action.ActionRepivot? || action.ActionSplit?
-  {
-    reveal_getActionToSplit();
-    var action := getActionToSplit(k, s, stack, slots, i);
-
-    if i == 0 {
-      //assert ValidAction(k, s, action);
-    } else {
-      if |s.cache[stack[i-1]].children.value| as uint64 < MaxNumChildren() as uint64 {
-        /*if |s.cache[stack[i]].buckets| as uint64 == 1 {
-          assert ValidAction(k, s, action);
-        } else {
-          assert ValidAction(k, s, action);
-        }*/
-      } else {
-        getActionToSplitValidAction(k, s, stack, slots, i-1);
-      }
-    }
-  }
-
-  lemma getActionToFlushValidAction(k: Constants, s: Variables, stack: seq<BT.G.Reference>, slots: seq<uint64>)
-  requires |stack| <= 40
-  requires ValidStackSlots(k, s, stack, slots)
-  requires Inv(k, s)
-  requires forall j | 0 <= j < |stack| :: stack[j] in s.ephemeralIndirectionTable
-  requires forall j | 0 <= j < |stack| - 1 :: s.cache[stack[j]].children.value[slots[j]] == stack[j+1]
-  requires forall j | 1 <= j < |stack| :: stack[j] != BT.G.Root()
-  decreases 0x1_0000_0000_0000_0000 - |stack|
-  ensures ValidAction(k, s, getActionToFlush(k, s, stack, slots))
-  {
-    reveal_getActionToFlush();
-    var action := getActionToFlush(k, s, stack, slots);
-
-    if |stack| as uint64 == 40 {
-    } else {
-      var ref := stack[|stack| as uint64 - 1];
-      var node := s.cache[ref];
-      if node.children.None? || |node.buckets| == MaxNumChildren() {
-        getActionToSplitValidAction(k, s, stack, slots, |stack| as uint64 - 1);
-      } else {
-        var (slot, slotWeight) := biggestSlot(node.buckets);
-        //if slotWeight >= FlushTriggerWeight() as uint64 || |node.children.value| as uint64 < 2 {
-          var childref := node.children.value[slot];
-          lemmaChildInGraph(k, s, ref, childref);
-          if childref in s.cache {
-            var child := s.cache[childref];
-            var childTotalWeight: uint64 := WeightBucketList(KMTable.ISeq(child.buckets)) as uint64;
-            var extraRootWeight: uint64 := if ref == BT.G.Root() then WeightBucket(s.rootBucket) as uint64 else 0;
-            if slotWeight + childTotalWeight + extraRootWeight <= MaxTotalBucketWeight() as uint64 {
-              assert ValidAction(k, s, action);
-            } else {
-              assume childref != BT.G.Root(); // TODO we need a way to show this
-              getActionToFlushValidAction(k, s, stack + [childref], slots + [slot]);
-            }
-          } else {
-            assert childref !in IVars(s).cache;
-            assert childref in IIndirectionTable(s.ephemeralIndirectionTable).graph;
-            assert childref in IIndirectionTable(s.ephemeralIndirectionTable).locs;
-            assert ValidAction(k, s, action);
-          }
-        //} else {
-        //  getActionToSplitValidAction(k, s, stack, slots, |stack| as uint64 - 1);
-        //}
-      }
-    }
-  }
-
-  lemma getActionToFlushWeightBounds(k: Constants, s: Variables, stack: seq<BT.G.Reference>, slots: seq<uint64>)
-  requires |stack| <= 40
-  requires ValidStackSlots(k, s, stack, slots)
-  requires Inv(k, s)
-  requires forall j | 0 <= j < |stack| :: stack[j] in s.ephemeralIndirectionTable
-  requires forall j | 0 <= j < |stack| - 1 :: s.cache[stack[j]].children.value[slots[j]] == stack[j+1]
-  requires forall j | 1 <= j < |stack| :: stack[j] != BT.G.Root()
-  decreases 0x1_0000_0000_0000_0000 - |stack|
-  ensures var action := getActionToFlush(k, s, stack, slots);
-      && ValidAction(k, s, action)
-      && (action.ActionFlush? ==>
-        && var parent := s.cache[action.parentref];
-        && var child := s.cache[parent.children.value[action.slot]];
-        (if action.parentref == BT.G.Root() then WeightBucket(s.rootBucket) else 0) +
-        WeightBucketList(KMTable.ISeq(child.buckets)) +
-        WeightBucket(KMTable.I(parent.buckets[action.slot])) <= MaxTotalBucketWeight()
-      )
-  {
-    reveal_getActionToFlush();
-    var action := getActionToFlush(k, s, stack, slots);
-
-    if |stack| as uint64 == 40 {
-    } else {
-      var ref := stack[|stack| as uint64 - 1];
-      var node := s.cache[ref];
-      if node.children.None? || |node.buckets| == MaxNumChildren() {
-        getActionToSplitValidAction(k, s, stack, slots, |stack| as uint64 - 1);
-      } else {
-        var (slot, slotWeight) := biggestSlot(node.buckets);
-        //if slotWeight >= FlushTriggerWeight() as uint64 || |node.children.value| as uint64 < 2 {
-          var childref := node.children.value[slot];
-          lemmaChildInGraph(k, s, ref, childref);
-          if childref in s.cache {
-            var child := s.cache[childref];
-            var childTotalWeight: uint64 := WeightBucketList(KMTable.ISeq(child.buckets)) as uint64;
-            var extraRootWeight: uint64 := if ref == BT.G.Root() then WeightBucket(s.rootBucket) as uint64 else 0;
-            if slotWeight + childTotalWeight + extraRootWeight <= MaxTotalBucketWeight() as uint64 {
-
-              assert extraRootWeight as int == (if action.parentref == BT.G.Root() then WeightBucket(s.rootBucket) else 0);
-              assert childTotalWeight as int == WeightBucketList(KMTable.ISeq(child.buckets));
-              assert slotWeight as int == WeightBucket(KMTable.I(node.buckets[action.slot]));
-
-              assert ValidAction(k, s, action);
-            } else {
-              assume childref != BT.G.Root(); // TODO we need a way to show this
-              getActionToFlushValidAction(k, s, stack + [childref], slots + [slot]);
-            }
-          } else {
-            assert childref !in IVars(s).cache;
-            assert childref in IIndirectionTable(s.ephemeralIndirectionTable).graph;
-            assert childref in IIndirectionTable(s.ephemeralIndirectionTable).locs;
-            assert ValidAction(k, s, action);
-          }
-        //} else {
-        //  getActionToSplitValidAction(k, s, stack, slots, |stack| as uint64 - 1);
-        //}
-      }
-    }
-  }
-
-
-  function {:opaque} runFlushPolicy(k: Constants, s: Variables, io: IO)
-  : (Variables, IO)
-  requires Inv(k, s)
-  requires io.IOInit?
+  requires io.initialized()
   requires s.Ready?
   requires BT.G.Root() in s.cache
+  modifies io
+  modifies s.ephemeralIndirectionTable.Repr
+  ensures WVars(s')
+  ensures (IVars(s'), IIO(io)) == ImplModelFlushPolicy.runFlushPolicy(Ic(k), old(IVars(s)), old(IIO(io)))
+  ensures forall r | r in s.ephemeralIndirectionTable.Repr :: fresh(r) || r in old(s.ephemeralIndirectionTable.Repr)
   {
+    ImplModelFlushPolicy.reveal_runFlushPolicy();
+
     var action := getActionToFlush(k, s, [BT.G.Root()], []);
-    getActionToFlushValidAction(k, s, [BT.G.Root()], []);
-
-    match action {
-      case ActionPageIn(ref) => (
-        PageInReq(k, s, io, ref)
-      )
-      case ActionSplit(parentref, slot) => (
-        var s' := doSplit(k, s, parentref, s.cache[parentref].children.value[slot], slot as int);
-        (s', io)
-      )
-      case ActionRepivot(ref) => (
-        var s' := repivotLeaf(k, s, ref, s.cache[ref]);
-        (s', io)
-      )
-      case ActionFlush(parentref, slot) => (
-        var s' := flush(k, s, parentref, slot as int, 
-            s.cache[parentref].children.value[slot],
-            s.cache[s.cache[parentref].children.value[slot]]);
-        (s', io)
-      )
-      case ActionGrow => (
-        var s' := grow(k, s);
-        (s', io)
-      )
-      case ActionEvict => (
-        (s, io) // TODO
-      )
-      case ActionFail => (
-        (s, io)
-      )
-    }
-  }
-
-  lemma runFlushPolicyCorrect(k: Constants, s: Variables, io: IO)
-  requires Inv(k, s)
-  requires io.IOInit?
-  requires s.Ready?
-  requires BT.G.Root() in s.cache
-  ensures var (s', io') := runFlushPolicy(k, s, io);
-    && WFVars(s')
-    && M.Next(Ik(k), IVars(s), IVars(s'), UI.NoOp, diskOp(io'))
-  {
-    var action := getActionToFlush(k, s, [BT.G.Root()], []);
-    getActionToFlushValidAction(k, s, [BT.G.Root()], []);
-
-    reveal_runFlushPolicy();
+    ImplModelFlushPolicy.getActionToFlushValidAction(Ic(k), IVars(s), [BT.G.Root()], []);
 
     match action {
       case ActionPageIn(ref) => {
-        PageInReqCorrect(k, s, io, ref);
+        s' := PageInReq(k, s, io, ref);
       }
       case ActionSplit(parentref, slot) => {
-        doSplitCorrect(k, s, parentref, s.cache[parentref].children.value[slot], slot as int);
+        s' := doSplit(k, s, parentref, s.cache[parentref].children.value[slot], slot as int);
       }
       case ActionRepivot(ref) => {
-        repivotLeafCorrect(k, s, ref, s.cache[ref]);
+        s' := repivotLeaf(k, s, ref, s.cache[ref]);
       }
       case ActionFlush(parentref, slot) => {
-        getActionToFlushWeightBounds(k, s, [BT.G.Root()], []);
-        flushCorrect(k, s, parentref, slot as int, 
+        s' := flush(k, s, parentref, slot as int, 
             s.cache[parentref].children.value[slot],
             s.cache[s.cache[parentref].children.value[slot]]);
       }
       case ActionGrow => {
-        growCorrect(k, s);
+        s' := grow(k, s);
       }
       case ActionEvict => {
-        assert noop(k, IVars(s), IVars(s));
+        s' := s;
       }
       case ActionFail => {
-        assert noop(k, IVars(s), IVars(s));
+        s' := s;
       }
     }
   }
-  */
 }
