disk-betree/UI.s.dfy
@@ -8,7 +8,7 @@ module {:extern} ValueWithDefault {
   type Value(==,!new) = s : seq<NativeTypes.byte> | |s| <= 1024
 	function method DefaultValue() : Value { [] }
 
-	function Len(v: Value) : nat { |v| }
+	function method Len(v: Value) : nat { |v| }
 
 	export S provides Value, DefaultValue, Len
 	export Internal reveals *
